## `PABS_CONV` {#PairRules.PABS_CONV}


```
PABS_CONV : conv -> conv
```



Applies a conversion to the body of a paired abstraction.


If `c` is a conversion that maps a term `t` to the theorem `|- t = t'`, then
the conversion `PABS_CONV c` maps abstractions of the form `\p.t` to theorems
of the form:
    
       |- (\p.t) = (\p.t')
    
That is, `ABS_CONV c "\p.t"` applies `p` to the body of the paired
abstraction `"\p.t"`.

### Failure

`PABS_CONV c tm` fails if `tm` is not a paired abstraction or if `tm` has the
form `"\p.t"` but the conversion `c` fails when applied to the term `t`.
The function returned by `ABS_CONV p` may also fail if the ML function
`c:term->thm` is not, in fact, a conversion (i.e. a function that maps a term
`t` to a theorem `|- t = t'`).

### Example

    
    - PABS_CONV SYM_CONV (Term `\(x,y). (1,2) = (x,y)`);
    > val it = |- (\(x,y). (1,2) = (x,y)) = (\(x,y). (x,y) = (1,2)) : thm
    



### See also

[`Conv.ABS_CONV`](#Conv.ABS_CONV), [`PairRules.PSUB_CONV`](#PairRules.PSUB_CONV)

