## `PEXT` {#PairRules.PEXT}


```
PEXT : (thm -> thm)
```



Derives equality of functions from extensional equivalence.


When applied to a theorem `A |- !p. t1 p = t2 p`,
the inference rule `PEXT` returns the theorem `A |- t1 = t2`.
    
        A |- !p. t1 p = t2 p
       ----------------------  PEXT          [where p is not free in t1 or t2]
            A |- t1 = t2
    



### Failure

Fails if the theorem does not have the form indicated above, or
if any of the component variables in the paired variable structure `p`
is free either of the functions `t1` or `t2`.

### Example

    
    - PEXT (ASSUME (Term `!(x,y). ((f:('a#'a)->'a) (x,y)) = (g (x,y))`));
    > val it =  [.] |- f = g : thm
    



### See also

[`Drule.EXT`](#Drule.EXT), [`Thm.AP_THM`](#Thm.AP_THM), [`PairRules.PETA_CONV`](#PairRules.PETA_CONV), [`Conv.FUN_EQ_CONV`](#Conv.FUN_EQ_CONV), [`PairRules.P_FUN_EQ_CONV`](#PairRules.P_FUN_EQ_CONV)

